src/3d/Options.fst
@@ -121,6 +121,8 @@ let z3_branch_depth : ref (option vstring) = alloc None
 
 let z3_options : ref (option vstring) = alloc None
 
+let z3_flight_name : ref (option vstring) = alloc None
+
 noeq
 type cmd_option_kind =
   | OptBool:
@@ -360,6 +362,7 @@ let (display_usage_2, compute_options_2, fstar_options) =
     CmdOption "equate_types" (OptList "an argument of the form A,B, to generate asserts of the form (A.t == B.t)" valid_equate_types equate_types_list) "Takes an argument of the form A,B and then for each entrypoint definition in B, it generates an assert (A.t == B.t) in the B.Types file, useful when refactoring specs, you can provide multiple equate_types on the command line" [];
     CmdOption "z3_branch_depth" (OptStringOption "nb" always_valid z3_branch_depth) "enumerate branch choices up to depth nb (default 0)" [];
     CmdOption "z3_diff_test" (OptStringOption "parser1,parser2" valid_equate_types z3_diff_test) "produce differential tests for two parsers" [];
+    CmdOption "z3_flight_name" (OptStringOption "ident" always_valid z3_flight_name) "C test case number <n> will be called witness<ident><n>" [];
     CmdOption "z3_executable" (OptStringOption "path/to/z3" always_valid z3_executable) "z3 executable for test case generation (default `z3`; does not affect verification of generated F* code)" [];
     CmdOption "z3_options" (OptStringOption "'options to z3'" always_valid z3_options) "command-line options to pass to z3 for test case generation (does not affect verification of generated F* code)" [];
     CmdOption "z3_skip_testcases_c" (OptBool no_produce_testcases_c) "skip generating test cases to <output directory>/testcases.c" [];
@@ -590,6 +593,11 @@ let get_z3_branch_depth () =
 
 let get_z3_options () : ML string = 
   match !z3_options with
+  | None -> ""
+  | Some s -> s
+
+let get_z3_flight_name () : ML string =
+  match !z3_flight_name with
   | None -> ""
   | Some s -> s
 
