src/3d/Options.fsti
@@ -82,6 +82,8 @@ val get_test_checker: unit -> ML (option string)
 
 val get_z3_branch_depth: unit -> ML nat
 
+val get_z3_flight_name: unit -> ML string
+
 val get_produce_testcases_c: unit -> ML bool
 
 val get_fstar_exe: unit -> ML string
