src/3d/Z3TestGen.fst
@@ -1367,14 +1367,17 @@ let rec print_witness_args_as_c
 
 let out_witness_len
   (out: (string -> ML unit))
+  (flight: string)
   (num: nat)
 : ML unit
 = out "witness";
+  out flight;
   out (string_of_int num);
   out "[0].len"
 
 let print_witness_call_as_c_aux
   (out: (string -> ML unit))
+  (flight: string)
   (validator_name: string)
   (arg_types: list (string & arg_type))
   (args: list string)
@@ -1385,9 +1388,10 @@ let print_witness_call_as_c_aux
   out "(";
   print_witness_args_as_c out arg_types args;
   out "&context, &TestErrorHandler, witness";
+  out flight;
   out (string_of_int num);
   out "[0].buf, ";
-  out_witness_len out num;
+  out_witness_len out flight num;
   out ", 0);"
 
 let pointer_elt_type_as_c (x: simple_arg_type true) : Tot (option string) =
@@ -1463,6 +1467,7 @@ let print_outparameters
     arg_types
 
 let alloc_copy_buffer
+  (flight: string)
   (wid: nat)
   (nblayers: nat)
   (arg_var: string)
@@ -1470,10 +1475,11 @@ let alloc_copy_buffer
 =
   Printf.sprintf
 "
-  copy_buffer_t _contents_%s = { .layers = witness%d, .count = %d, .cur = 0U };
+  copy_buffer_t _contents_%s = { .layers = witness%s%d, .count = %d, .cur = 0U };
   EVERPARSE_COPY_BUFFER_T %s = (void* ) &_contents_%s;
 "
   arg_var
+  flight
   wid
   nblayers
   arg_var
@@ -1483,6 +1489,7 @@ let print_witness_call_as_c
   (out: (string -> ML unit))
   (p: prog)
   (positive: bool)
+  (flight: string)
   (validator_name: string)
   (arg_types: list (string & arg_type))
   (args: list string)
@@ -1497,23 +1504,23 @@ let print_witness_call_as_c
   List.iter
     (fun arg_ty ->
       match arg_ty with
-      | (arg_var, ArgCopyBuffer) -> out (alloc_copy_buffer num nblayers arg_var)
+      | (arg_var, ArgCopyBuffer) -> out (alloc_copy_buffer flight num nblayers arg_var)
       | (arg_var, ArgPointer ty) -> out (alloc_ptr_arg arg_var ty)
       | (_, ArgSimple _) -> ()
     )
     arg_types;
   out "
     uint64_t output = ";
-  print_witness_call_as_c_aux out validator_name arg_types args num;
+  print_witness_call_as_c_aux out flight validator_name arg_types args num;
   out "
     printf(\"  // ";
-  print_witness_call_as_c_aux out validator_name arg_types args num;
+  print_witness_call_as_c_aux out flight validator_name arg_types args num;
   out " // \");
     BOOLEAN result = !EverParseIsError(output);
     BOOLEAN consumes_all_bytes_if_successful = true;
     if (result) {
       consumes_all_bytes_if_successful = (output == ";
-  out_witness_len out num;
+  out_witness_len out flight num;
   out ");
       result = consumes_all_bytes_if_successful;
     }
@@ -1538,13 +1545,14 @@ let print_witness_call_as_c
 
 let print_witness_layer_as_c_aux
   (out: (string -> ML unit))
+  (flight: string)
   (witness: Seq.seq int)
   (len: int { len == Seq.length witness })
   (num: nat)
   (lid: int)
 : ML string
 =
-  let layer_name = "witness" ^ string_of_int num ^ "_" ^ string_of_int lid in
+  let layer_name = "witness" ^ flight ^ string_of_int num ^ "_" ^ string_of_int lid in
   out "  uint8_t ";
   if len > 0
   then begin
@@ -1569,6 +1577,7 @@ let print_witness_layer_as_c_aux
 
 let print_witness_as_c_aux
   (out: (string -> ML unit))
+  (flight: string)
   (witness: Seq.seq (Seq.seq int))
   (len: int { len == Seq.length witness })
   (num: nat)
@@ -1580,7 +1589,7 @@ let print_witness_as_c_aux
     else begin
       let w = Seq.index witness i in
       let wlen = Seq.length w in
-      let layer_name = print_witness_layer_as_c_aux out w wlen num i in
+      let layer_name = print_witness_layer_as_c_aux out flight w wlen num i in
       let layer = "{ .buf = " ^ layer_name ^ ", .len = " ^ string_of_int wlen ^ "}" in
       let accu' =
         if accu = ""
@@ -1592,6 +1601,7 @@ let print_witness_as_c_aux
   in
   let layers = aux "" 0 in
   out "  witness_layer_t witness";
+  out flight;
   out (string_of_int num);
   out "[";
   out (string_of_int len);
@@ -1601,16 +1611,17 @@ let print_witness_as_c_aux
 
 let print_witness_as_c_gen
   (out: (string -> ML unit))
+  (flight: string)
   (witness: Seq.seq (Seq.seq int))
   (f: (len: int { len == Seq.length witness }) -> ML unit)
   (num: nat)
 : ML unit
 = let len = Seq.length witness in
   out "{\n";
-  print_witness_as_c_aux out witness len num;
+  print_witness_as_c_aux out flight witness len num;
   out "
   printf(\"";
-  print_witness_as_c_aux out witness len num;
+  print_witness_as_c_aux out flight witness len num;
   out "\\n\");
 ";
   f len;
@@ -1656,6 +1667,7 @@ let print_witness_as_c
   (out: (string -> ML unit))
   (p: prog)
   (positive: bool)
+  (flight: string)
   (validator_name: string)
   (arg_types: list (string & arg_type))
   (counter: ref nat)
@@ -1664,16 +1676,17 @@ let print_witness_as_c
 : ML unit
 = let num = incr counter in
   write_witness_to_file witness (fun i -> mk_output_filename num out_dir ((if positive then "POS." else "NEG.") ^ string_of_int i ^ "." ^ validator_name) args);
-  print_witness_as_c_gen out witness (fun len ->
+  print_witness_as_c_gen out flight witness (fun len ->
     if len = 0
     then failwith "print_witness_as_c: no witness layers. This should not happen.";
-    print_witness_call_as_c out p positive validator_name arg_types args num len
+    print_witness_call_as_c out p positive flight validator_name arg_types args num len
   ) num
 
 let print_diff_witness_as_c
   (out_dir: string)
   (out: (string -> ML unit))
   (p: prog)
+  (flight: string)
   (validator_name1: string)
   (validator_name2: string)
   (arg_types: list (string & arg_type))
@@ -1683,11 +1696,11 @@ let print_diff_witness_as_c
 : ML unit
 = let num = incr counter in
   write_witness_to_file witness (fun i -> mk_output_filename num out_dir ("POS." ^ string_of_int i ^ "." ^ validator_name1 ^ ".NEG." ^ validator_name2) args);
-  print_witness_as_c_gen out witness (fun len ->
+  print_witness_as_c_gen out flight witness (fun len ->
     if len = 0
     then failwith "print_witness_as_c: no witness layers. This should not happen.";
-    print_witness_call_as_c out p true validator_name1 arg_types args num len;
-    print_witness_call_as_c out p false validator_name2 arg_types args num len
+    print_witness_call_as_c out p true flight validator_name1 arg_types args num len;
+    print_witness_call_as_c out p false flight validator_name2 arg_types args num len
   )
   num
 
@@ -2006,7 +2019,7 @@ let cout_test_probe_functions
     )
     prog
 
-let do_test (out_dir: string) (out_file: option string) (z3: Z3.z3) (prog: prog) (name1: string) (nbwitnesses: int) (depth: nat) (pos: bool) (neg: bool) : ML unit =
+let do_test (out_dir: string) (out_file: option string) (z3: Z3.z3) (flight: string) (prog: prog) (name1: string) (nbwitnesses: int) (depth: nat) (pos: bool) (neg: bool) : ML unit =
   let def = List.assoc name1 prog in
   begin match def with
   | Some (ProgDef _ _) -> ()
@@ -2032,7 +2045,7 @@ let do_test (out_dir: string) (out_file: option string) (z3: Z3.z3) (prog: prog)
   let tasks =
     begin
       if pos
-      then [print_witness_as_c out_dir cout prog true validator_name args counter, (fun _ -> (
+      then [print_witness_as_c out_dir cout prog true flight validator_name args counter, (fun _ -> (
         FStar.IO.print_string (Printf.sprintf ";; Positive test witnesses for %s\n" name1);
         mk_get_positive_test_witness name1 sargs
       ))]
@@ -2040,7 +2053,7 @@ let do_test (out_dir: string) (out_file: option string) (z3: Z3.z3) (prog: prog)
     end `List.Tot.append`
     begin
       if neg
-      then [print_witness_as_c out_dir cout prog false validator_name args counter, (fun _ -> (
+      then [print_witness_as_c out_dir cout prog false flight validator_name args counter, (fun _ -> (
         FStar.IO.print_string (Printf.sprintf ";; Negative test witnesses for %s\n" name1);
         mk_get_negative_test_witness name1 sargs
       ))]
@@ -2067,12 +2080,12 @@ let mk_get_diff_test_witness (name1: string) (l: list arg_type) (name2: string) 
   (mk_state "(state-witness-size 0)" "0" "0" "1" "-1")
 
 let do_diff_test_for
-  (out_dir: string) (counter: ref nat) (cout: string -> ML unit) (z3: Z3.z3) (prog: prog) name1 name2 (args: list (string & arg_type)) (nargs: nat { nargs == count_args (List.Tot.map snd args) }) validator_name1 validator_name2 nbwitnesses depth =
+  (out_dir: string) (counter: ref nat) (cout: string -> ML unit) (z3: Z3.z3) (flight: string) (prog: prog) name1 name2 (args: list (string & arg_type)) (nargs: nat { nargs == count_args (List.Tot.map snd args) }) validator_name1 validator_name2 nbwitnesses depth =
   FStar.IO.print_string (Printf.sprintf ";; Witnesses that work with %s but not with %s\n" name1 name2);
   let sargs = List.Tot.map snd args in
-  witnesses_for z3 name1 sargs nargs ([print_diff_witness_as_c out_dir cout prog validator_name1 validator_name2 args counter, (fun _ -> mk_get_diff_test_witness name1 sargs name2)]) nbwitnesses depth
+  witnesses_for z3 name1 sargs nargs ([print_diff_witness_as_c out_dir cout prog flight validator_name1 validator_name2 args counter, (fun _ -> mk_get_diff_test_witness name1 sargs name2)]) nbwitnesses depth
 
-let do_diff_test (out_dir: string) (out_file: option string) (z3: Z3.z3) (prog: prog) name1 name2 nbwitnesses depth =
+let do_diff_test (out_dir: string) (out_file: option string) (z3: Z3.z3) (flight: string) (prog: prog) name1 name2 nbwitnesses depth =
   let def = List.assoc name1 prog in
   begin match def with
   | Some (ProgDef _ _) -> ()
@@ -2104,8 +2117,8 @@ let do_diff_test (out_dir: string) (out_file: option string) (z3: Z3.z3) (prog: 
   int main(void) {
 ";
   let counter = alloc 0 in
-  do_diff_test_for out_dir counter cout z3 prog name1 name2 args nargs validator_name1 validator_name2 nbwitnesses depth;
-  do_diff_test_for out_dir counter cout z3 prog name2 name1 args nargs validator_name2 validator_name1 nbwitnesses depth;
+  do_diff_test_for out_dir counter cout z3 flight prog name1 name2 args nargs validator_name1 validator_name2 nbwitnesses depth;
+  do_diff_test_for out_dir counter cout z3 flight prog name2 name1 args nargs validator_name2 validator_name1 nbwitnesses depth;
   cout "  return 0;
   }
 "
